Examples/Lexer.lean
@@ -1,0 +1,57 @@
+import PrimParser
+
+open Parser Parser.Char
+
+inductive Tk where
+  | num (n : Nat)
+  | plus
+  | minus
+  | times
+  | lparen
+  | rparen
+  deriving Repr, BEq, Inhabited
+
+namespace Lex
+
+def one : StringParser conditional Tk :=
+  oneOf (
+    (Tk.num <$>ᵍ nat) ::₁
+    [ Tk.plus   <$ᵍ char '+'
+    , Tk.minus  <$ᵍ char '-'
+    , Tk.times  <$ᵍ char '*'
+    , Tk.lparen <$ᵍ char '('
+    , Tk.rparen <$ᵍ char ')' ])
+
+def lex : StringParser flexible (Array Tk) := gdo
+  whitespace
+  let ts ← many (lexeme one)
+  return ts.toArray
+
+def sym (t : Tk) : TokenParser Tk conditional PUnit := skipSatisfy (· == t)
+
+def num : TokenParser Tk conditional Nat :=
+  token fun
+    | .num n => some n
+    | _ => none
+
+def addOp : TokenParser Tk conditional (Nat → Nat → Nat) :=
+  (· + ·) <$ᵍ sym .plus <|> (· - ·) <$ᵍ sym .minus
+
+def mulOp : TokenParser Tk conditional (Nat → Nat → Nat) :=
+  (· * ·) <$ᵍ sym .times
+
+def eval : TokenParser Tk conditional Nat :=
+  fix fun self =>
+    let atom := num <|> rawBracket (sym .lparen) (sym .rparen) self
+    chainl1 addOp (chainl1 mulOp atom)
+
+def evalAll : TokenParser Tk conditional Nat := gdo
+  let v ← eval
+  eof
+  return v
+
+def run (s : String) : Option Nat := do
+  let ts ← lex.runOption s
+  (evalAll.runOn (Input.ofArray ts)).toOption
+
+end Lex
