PrimParser/Buffer.lean
@@ -1,0 +1,58 @@
+import Mathlib.Order.Fin.Basic
+
+/-- `σ` is a sequence of tokens of type `τ` -/
+class Buffer (σ τ : Type) where
+  size : σ → Nat
+  nil : σ
+  width : τ → Nat
+  width_pos : ∀ t, 0 < width t
+  nextTok : σ → (remaining : Nat) → Option τ
+  nextTok_le : ∀ {s n t}, nextTok s n = some t → width t ≤ n
+
+namespace Buffer
+
+variable {σ τ : Type} [Buffer σ τ]
+
+@[simp] theorem nextTok_zero (s : σ) : nextTok (τ := τ) s 0 = none := by
+  cases h : nextTok (τ := τ) s 0 with
+  | none => rfl
+  | some t => have := nextTok_le h; have := width_pos (σ := σ) t; omega
+
+theorem sub_width_lt {s : σ} {n : Nat} {t : τ}
+  (h : nextTok s n = some t)
+  : n - width σ t < n := by
+  have := nextTok_le h
+  have := width_pos (σ := σ) t
+  omega
+
+instance : Buffer ByteArray Char where
+  size := ByteArray.size
+  nil := .empty
+  width := Char.utf8Size
+  width_pos := Char.utf8Size_pos
+  nextTok s n := s.utf8DecodeChar? (s.size - n)
+  nextTok_le h := by
+    have := ByteArray.le_size_of_utf8DecodeChar?_eq_some h
+    omega
+
+@[simp] theorem size_byteArray (b : ByteArray) : size Char b = b.size := rfl
+@[simp] theorem width_byteArray (c : Char) : width ByteArray c = c.utf8Size := rfl
+@[simp] theorem nextTok_byteArray (b : ByteArray) (n : Nat)
+  : nextTok (τ := Char) b n = b.utf8DecodeChar? (b.size - n) := rfl
+
+instance {τ : Type} : Buffer (Array τ) τ where
+  size := Array.size
+  nil := #[]
+  width _ := 1
+  width_pos _ := by simp
+  nextTok a n := a[a.size - n]?
+  nextTok_le h := by
+    have := Array.getElem?_eq_some_iff.mp h |>.fst
+    omega
+
+@[simp] theorem size_array {τ : Type} (a : Array τ) : size τ a = a.size := rfl
+@[simp] theorem width_array {τ : Type} (t : τ) : width (Array τ) t = 1 := rfl
+@[simp] theorem nextTok_array {τ : Type} (a : Array τ) (n : Nat)
+  : nextTok a n = a[a.size - n]? := rfl
+
+end Buffer
